Smart constructors, optimize 0+e etc.

Imp/Expr/Optimize.lean
@@ -3,40 +3,57 @@ import Imp.Expr.Eval
 
 namespace Imp.Expr
 
+/-- Smart constructor that optimizes unary operations. NB: Same type as `Expr.unop` -/
+def unopOpt : UnOp → Expr → Expr
+  | uop, .const i =>
+    if let some v := uop.apply i then .const v
+    else .unop uop (.const i)
+  | uop, e => .unop uop e
+
+/-- Smart constructor that optimizes binary operations. NB: Same type as `Expr.op` -/
+def opOpt : BinOp → Expr → Expr → Expr
+  | bop, .const i, .const i' =>
+    if let some v := bop.apply i i' then .const v
+    else .op bop (.const i) (.const i')
+  | .plus, .const 0, e => e
+  | .plus, e, const 0 => e
+  | .times, .const 1, e => e
+  | .times, e, const 1 => e
+  | bop, e1, e2 => .op bop e1 e2
+
 /--
 Optimizes an expression by folding constants.
 -/
 def optimize : Expr → Expr
   | .const i => .const i
   | .var x => .var x
-  | .unop uop e =>
-    match optimize e with
-    | .const i =>
-      if let some v := uop.apply i then .const v
-      else .unop uop (.const i)
-    | e' => .unop uop e'
-  | .op bop e1 e2 =>
-    match optimize e1, optimize e2 with
-    | .const i, .const i' =>
-      if let some v := bop.apply i i' then .const v
-      else .op bop (.const i) (.const i')
-    | e1', e2' => .op bop e1' e2'
+  | .unop uop e => .unopOpt uop (optimize e)
+  | .op bop e1 e2 => .opOpt bop (optimize e1) (optimize e2)
+
+/-- Correctness of the `.unOpt` smart constructor -/
+@[simp]
+theorem unopOpt_ok : (Expr.unopOpt uop e).eval σ = (Expr.unop uop e).eval σ := by
+  unfold Expr.unopOpt
+  split <;> simp [eval, *]
+  · split <;> simp [eval, *]
+
+@[simp] theorem BinOp.apply_plus_0_left  : BinOp.plus.apply (0#32) v = v := by simp [BinOp.apply]
+@[simp] theorem BinOp.apply_plus_0_right : BinOp.plus.apply v (0#32) = v := by simp [BinOp.apply]
+@[simp] theorem BinOp.apply_mul_1_left   : BinOp.times.apply (1#32) v = v := by simp [BinOp.apply]
+@[simp] theorem BinOp.apply_mul_1_right  : BinOp.times.apply v (1#32) = v := by simp [BinOp.apply]
+
+/-- Correctness of the `.opOpt` smart constructor -/
+@[simp]
+theorem opOpt_ok : (Expr.opOpt bop e1 e2).eval σ = (Expr.op bop e1 e2).eval σ := by
+  unfold Expr.opOpt
+  split <;> simp [eval, *]
+  · split <;> simp [eval, *]
 
 /--
 Optimization doesn't change the meaning of any expression
 -/
 theorem optimize_ok (e : Expr) : e.eval σ = e.optimize.eval σ := by
-  induction e <;> simp [optimize]
-  case unop uop e ih =>
-    split <;> simp [eval, *]
-    split
-    · simp [eval, *]
-    · simp [eval]
-  case op bop e1 e2 ih1 ih2 =>
-    split <;> simp [eval, *]
-    split
-    · simp [eval, *]
-    · simp [eval]
+  induction e <;> simp [optimize, eval, *]
 
 /--
 Optimization doesn't change the meaning of any expression
